lean/src/r_correct_theorem.lean
@@ -184,15 +184,15 @@ begin
 end
 -/
 
-lemma gdt_branch_replace_left_env { gdt1 gdt1' gdt2: option Gdt } { env: Env }
+lemma gdt_build_branch_replace_left_env { gdt1 gdt1' gdt2: option Gdt } { env: Env }
     (h: gdt_eval_option gdt1 env = gdt_eval_option gdt1' env):
-    gdt_eval_option (gdt_branch gdt1 gdt2) env = gdt_eval_option (gdt_branch gdt1' gdt2) env :=
+    gdt_eval_option (gdt_build_branch gdt1 gdt2) env = gdt_eval_option (gdt_build_branch gdt1' gdt2) env :=
 begin
     cases gdt1;
     cases gdt1';
     cases gdt2;
     
-    finish [gdt_branch, gdt_eval_option, gdt_eval, gdtx],
+    finish [gdt_build_branch, gdt_eval_option, gdt_eval, gdtx],
 end
 
 def 𝒰'option: option Gdt → Φ
@@ -200,9 +200,9 @@ def 𝒰'option: option Gdt → Φ
 | none := Φ.true
 
 
-lemma gdt_branch_replace_right_env { gdt1 gdt2 gdt2': option Gdt } { env: Env }
+lemma gdt_build_branch_replace_right_env { gdt1 gdt2 gdt2': option Gdt } { env: Env }
     (h: (Φ_eval (𝒰'option gdt1) env) → gdt_eval_option gdt2 env = gdt_eval_option gdt2' env):
-    gdt_eval_option (gdt_branch gdt1 gdt2) env = gdt_eval_option (gdt_branch gdt1 gdt2') env :=
+    gdt_eval_option (gdt_build_branch gdt1 gdt2) env = gdt_eval_option (gdt_build_branch gdt1 gdt2') env :=
 begin
     cases gdt1,
     case option.some {
@@ -218,10 +218,10 @@ begin
             
             all_goals {
                 try {
-                    simp [gdt_eval_option, gdt_branch, 𝒰'option, gdt_eval, gdt_eval._match_1, c],
+                    simp [gdt_eval_option, gdt_build_branch, 𝒰'option, gdt_eval, gdt_eval._match_1, c],
                 },
                 try {
-                    simp [gdt_eval_option, gdt_branch, 𝒰'option, gdt_eval, gdt_eval._match_1, c] at h,
+                    simp [gdt_eval_option, gdt_build_branch, 𝒰'option, gdt_eval, gdt_eval._match_1, c] at h,
                 },
             },
             all_goals {
@@ -236,13 +236,13 @@ begin
             cases gdt2';
 
 
-            simp [gdt_branch, gdt_eval_option, c],
+            simp [gdt_build_branch, gdt_eval_option, c],
         }
     },
     case option.none {
         cases gdt2';
         cases gdt2;
-        finish [gdt_eval_option, gdt_branch, 𝒰'option],
+        finish [gdt_eval_option, gdt_build_branch, 𝒰'option],
     },
 end
 
@@ -266,6 +266,24 @@ begin
         rw map_ant at h,
         use ant_tr1,
         use ant_tr2,
+        finish,
+    },
+end
+
+lemma inverse_map_ant_diverge { α β: Type } { ant: Ant α } { b: β } { a: Ant β } { f: α → β }
+    (h: map_ant f ant = Ant.diverge b a):
+    ∃ ant_a: α, ∃ ant_ant: Ant α,
+        ant = Ant.diverge ant_a ant_ant ∧ b = f ant_a ∧ a = map_ant f ant_ant :=
+begin
+    cases ant,
+    case Ant.leaf { finish, },
+    case Ant.diverge {
+        rw map_ant at h,
+        use ant_a,
+        use ant_tr,
+        finish,
+    },
+    case Ant.branch {
         finish,
     },
 end
@@ -358,37 +376,80 @@ begin
 end
 
 
-def is_strict (f: Φ → Φ) (env: Env) := ∀ ty: Φ, Φ_eval ty env = tt → Φ_eval (f ty) env = tt
 
-
-lemma xgrd_in_strictness { f: Φ → Φ } { env env': Env } { grd: XGrd }
-    (h1: is_strict f env) (h2: xgrd_eval grd env = some env'):
-        is_strict (f ∘ Φ.xgrd_in grd) env' :=
+lemma grd_eval_xgrd_some { grd: XGrd } { tr: Gdt } { env env': Env }
+    (h: xgrd_eval grd env = some env'):
+    gdt_eval (Gdt.grd (Grd.xgrd grd) tr) env = gdt_eval tr env' :=
 begin
-    rw is_strict,
-    intro ty,
-    intro p,
-    rw function.comp,
-    simp,
-
-    rw is_strict at h1,
-    specialize h1 (Φ.xgrd_in grd ty),
-    simp [Φ_eval, h2, p] at h1,
-    simp [h1],
+    simp [gdt_eval, h],
 end
 
---  is_strict (f ∘ Φ.xgrd_in gdt_grd) env 
+lemma grd_eval_xgrd_none { grd: XGrd } { tr: Gdt } { env: Env }
+    (h: xgrd_eval grd env = none):
+    gdt_eval (Gdt.grd (Grd.xgrd grd) tr) env = Result.no_match :=
+begin
+    simp [gdt_eval, h],
+end
+
+lemma grd_eval_option_xgrd_some { grd: XGrd } { tr: option Gdt } { env env': Env }
+    (h: xgrd_eval grd env = some env'):
+    gdt_eval_option (gdt_build_grd (Grd.xgrd grd) tr) env = gdt_eval_option tr env' :=
+begin
+    cases tr;
+    simp [gdt_eval_option, gdt_build_grd, gdt_eval, h],
+end
+
+lemma grd_eval_option_xgrd_none { grd: XGrd } { tr: option Gdt } { env }
+    (h: xgrd_eval grd env = none):
+    gdt_eval_option (gdt_build_grd (Grd.xgrd grd) tr) env = Result.no_match :=
+begin
+    cases tr;
+    simp [gdt_eval_option, gdt_build_grd, gdt_eval, h],
+end
+
+lemma grd_eval_bang_is_not_bottom { tr: Gdt } { env: Env } { var: Var }
+    (h: is_bottom var env = ff):
+    gdt_eval (Gdt.grd (Grd.bang var) tr) env = gdt_eval tr env :=
+begin
+    simp [gdt_eval, h],
+end
+
+lemma grd_eval_bang_is_bottom { tr: Gdt } { env: Env } { var: Var }
+    (h: is_bottom var env = tt):
+    gdt_eval (Gdt.grd (Grd.bang var) tr) env = Result.diverged :=
+begin
+    simp [gdt_eval, h],
+end
+
+lemma grd_eval_option_bang_is_not_bottom { tr: option Gdt } { env: Env } { var: Var }
+    (h: is_bottom var env = ff):
+    gdt_eval_option (gdt_build_grd (Grd.bang var) tr) env = gdt_eval_option tr env :=
+begin
+    cases tr;
+    simp [gdt_eval, gdt_eval_option, gdt_build_grd, h],
+end
+
+lemma grd_eval_option_bang_is_bottom { tr: option Gdt } { env: Env } { var: Var }
+    (h: is_bottom var env = tt):
+    gdt_eval_option (gdt_build_grd (Grd.bang var) tr) env =
+        if tr.is_some then Result.diverged else Result.no_match :=
+begin
+    cases tr;
+    simp [gdt_eval, gdt_eval_option, gdt_build_grd, h],
+end
+
 
 lemma r_correct_2
     (is_empty: Gs)
     (gdt: Gdt) (gdt_disjoint: disjoint_leaves gdt)
-    (env: Env) (f: Φ → Φ) (f_prop: is_strict f env)
-    (ant: Ant Φ) (ant_def: ant_eval_all ant env = ant_eval_all (map_ant f (𝒜' gdt)) env)
+    (env ant_env: Env)
+    (ant: Ant Φ) (ant_def: ant_eval_all ant ant_env = ant_eval_all (𝒜' gdt) env)
     (r: LeafPartition) (r_def: r = R is_empty.val ant):
 
         gdt_eval_option (gdt_remove_leaves r.red.to_finset gdt) env = gdt_eval gdt env :=
 begin
-    induction gdt generalizing f r ant env,
+    induction gdt generalizing r ant env ant_env,
+
 
     case Gdt.grd {
         rw disjoint_leaves at gdt_disjoint,
@@ -400,44 +461,171 @@ begin
         case Grd.xgrd {
 
             rw [𝒜'] at ant_def,
-            rw map_ant_associative at ant_def,
-            specialize gdt_ih (f ∘ Φ.xgrd_in gdt_grd) r ant,
-
-            rw gdt_eval, -- todo
-
-            cases c: xgrd_eval gdt_grd env,
+            
+            cases c: xgrd_eval gdt_grd env with env',
 
             case option.some {
-                rw gdt_eval._match_2,
-                rw gdt_remove_leaves,
+                -- todo
+                unfold ant_eval_all at ant_def,
+                rw map_ant_associative at ant_def,
+                rw function.comp at ant_def,
+                unfold Φ_eval at ant_def,
+                rw c at ant_def,
+                unfold Φ_eval._match_1 at ant_def,
+                rw ←ant_eval_all at ant_def,
+                rw ←ant_eval_all at ant_def,
+                
+                specialize gdt_ih r ant env' ant_env ant_def r_def,
+                
+                
+                rw [gdt_remove_leaves, grd_eval_xgrd_some c, grd_eval_option_xgrd_some c],
+                exact gdt_ih,
+            },
+
+            case option.none {
+                rw [gdt_remove_leaves, grd_eval_option_xgrd_none c, grd_eval_xgrd_none c],
             },
         },
 
         case Grd.bang {
+            rw [𝒜'] at ant_def,
+            unfold ant_eval_all at ant_def,
+            unfold map_ant at ant_def,
+            rw ←ant_eval_all at ant_def,
+            rw map_ant_associative at ant_def,
+            rw function.comp at ant_def,
+            unfold Φ_eval at ant_def,
 
+            
+            
+            replace ant_def := inverse_map_ant_diverge ant_def,
+            cases ant_def with ant_a ant_def,
+            cases ant_def with ant_ant ant_def,
+            cases ant_def with ant_def ant_h1,
+            cases ant_h1 with ant_h1 ant_h2,
+
+            simp at ant_h1,
+
+            rw ant_def at r_def,
+            --rw R at r_def,
+            --rw map_ant at r_def,
+            --rw R' at r_def,
+            --rw ←R at r_def,
+
+            cases c: is_bottom gdt_grd env,
+            case bool.ff {
+                rw c at ant_h2,
+                simp at ant_h2,
+                rw ←ant_eval_all at ant_h2,
+                rw ←ant_eval_all at ant_h2,
+
+                
+                set r' := R is_empty.val ant_ant with r'_def,
+
+
+                specialize gdt_ih r' ant_ant env ant_env (eq.symm ant_h2) r'_def,
+
+
+                have y := R_diverge ant_a (eq.symm r'_def),
+
+                cases y,
+                case or.inl {
+                    cases y with hr y,
+                    cases y with rs y,
+                    cases y with y1 y,
+                    cases y with y2 y,
+                    rw y at r_def,
+                    rw r_def,
+                    simp,
+                    rw y2 at gdt_ih,
+                    simp at gdt_ih,
+                    rw grd_eval_bang_is_not_bottom c,
+                    rw ←gdt_ih,
+                    rw gdt_remove_leaves,
+                    rw grd_eval_option_bang_is_not_bottom c,
+                    sorry,
+                },
+
+                case or.inr {
+                    cases y with y1 y,
+                    rw y at r_def,
+                    rw ← r_def at gdt_ih,
+                    rw grd_eval_bang_is_not_bottom c,
+                    rw gdt_remove_leaves,
+                    rw grd_eval_option_bang_is_not_bottom c,
+                    exact gdt_ih,
+                },
+            },
+
+            case bool.tt {
+                rw c at ant_h2,
+                simp at ant_h2,
+
+                set r' := R is_empty.val ant_ant with r'_def,
+
+                rw grd_eval_bang_is_bottom c,
+
+                have y := R_diverge ant_a (eq.symm r'_def),
+
+                rw gdt_remove_leaves,
+                rw grd_eval_option_bang_is_bottom c,
+
+                suffices : (gdt_remove_leaves r.red.to_finset gdt_tr).is_some = tt,
+                simp [this],
+
+                cases y,
+
+                case or.inl {
+                    cases y with hr y,
+                    cases y with rs y,
+                    cases y with y1 y,
+                    cases y with y2 y,
+                    sorry,
+                },
+
+                case or.inr {
+                    cases y with y1 y,
+                    rw y at r_def,
+                    rw r_def,
+                    cases y1 with x y,
+                    rw c at ant_h1,
+                    finish [is_empty_implies_eval_false x],
+                    sorry,
+                }
+
+                -- to show: ∃ x ∈ gdt_leaves ant_grd \ r.red 
+            },
+
+            
         },
     },
 
-/-
+
     case Gdt.leaf {
         simp [gdt_eval],
-        simp [𝒜', map_ant] at ha,
+        simp [𝒜', map_ant] at ant_def,
         
-        have ha := inverse_map_ant_leaf ha,
+        have ha := inverse_map_ant_leaf ant_def,
         cases ha with ty ha,
         cases ha with ha1 ha2,
-        rw ha1 at hr,
-        rw R at hr,
-        rw map_ant at hr,
-        rw R' at hr,
+        rw ha1 at r_def,
+        rw R at r_def,
+        rw map_ant at r_def,
+        rw R' at r_def,
 
         cases c: is_empty.val ty,
-        { simp [hr, gdt_eval_option, gdt_eval, c], },
+        { simp [r_def, gdt_eval_option, gdt_eval, c], },
         { finish [is_empty_implies_eval_false c], },
     },
 
     case Gdt.branch {
         -- branch to top
+
+
+        have ha := ant_def,
+        have hr := r_def,
+        have d := gdt_disjoint,
+
         rw 𝒜' at ha,
         rw ant_eval_all at ha,
         rw ant_eval_all at ha,
@@ -469,14 +657,14 @@ begin
         cases d with d_tr2 d,
         
 
-        specialize gdt_ih_tr1 d_tr1 r1 ant1,
+        specialize gdt_ih_tr1 d_tr1 r1 ant1 env ant_env,
         replace gdt_ih_tr1 := gdt_ih_tr1 (eq.symm ha2) r1_eq,
 
 
         rw gdt_remove_leaves,
  
         have grd1_ant1_leaves_eq: ant_leaves ant1 = gdt_leaves gdt_tr1, {
-            rw ←map_leaves_id _ (λ ty, Φ_eval ty env),
+            rw ←map_leaves_id _ (λ ty, Φ_eval ty ant_env),
             rw ←ant_eval_all,
             rw ←ha2,
             simp [gdt_leaves_eq_ant_leaves, map_leaves_id, ant_eval_all],
@@ -498,7 +686,7 @@ begin
                 simp [r2.red.to_finset.subset_union_left, R_partition r2_eq, x],
             },
             have grd2_ant2_leaves_eq: ant_leaves ant2 = gdt_leaves gdt_tr2, {
-                rw ←map_leaves_id _ (λ ty, Φ_eval ty env),
+                rw ←map_leaves_id _ (λ ty, Φ_eval ty ant_env),
                 rw ←ant_eval_all,
                 rw ←ha3,
                 simp [gdt_leaves_eq_ant_leaves, map_leaves_id, ant_eval_all],
@@ -526,7 +714,7 @@ begin
 
         rw this at gdt_ih_tr1,
 
-        rw gdt_branch_replace_left_env gdt_ih_tr1,
+        rw gdt_build_branch_replace_left_env gdt_ih_tr1,
 
         clear gdt_ih_tr1,
         clear this,
@@ -554,7 +742,7 @@ begin
             rw ←ant_eval_all at ha3,
             rw ←ant_eval_all at ha3,
             rw ←R at r2_eq,
-            specialize gdt_ih_tr2 d_tr2 r2 ant2,
+            specialize gdt_ih_tr2 d_tr2 r2 ant2 env ant_env,
             replace gdt_ih_tr2 := gdt_ih_tr2 (eq.symm ha3) r2_eq,
             rw gdt_eval_option,
             rw ← gdt_ih_tr2,
@@ -571,7 +759,7 @@ begin
                     simp [r1.red.to_finset.subset_union_left, R_partition r1_eq, x],
                 },
                 have grd1_ant1_leaves_eq: ant_leaves ant1 = gdt_leaves gdt_tr1, {
-                    rw ←map_leaves_id _ (λ ty, Φ_eval ty env),
+                    rw ←map_leaves_id _ (λ ty, Φ_eval ty ant_env),
                     rw ←ant_eval_all,
                     rw ←ha2,
                     simp [gdt_leaves_eq_ant_leaves, map_leaves_id, ant_eval_all],
@@ -596,71 +784,10 @@ begin
             rw this,
         end,
 
-        rw gdt_branch_replace_right_env p,
-        simp [gdt_branch, gdt_eval_option],
-    },
-    -/
-end
-
-
-/-
-
-
-
-lemma r_correct_2
-    (is_empty: Gs) (gdt: Gdt) (r: LeafPartition) (ant: Ant Φ)
-    (ha: ant_eval_all ant = ant_eval_all (𝒜' gdt))
-    (hr: r = R is_empty.val ant):
-        gdt_eval_option (gdt_remove_leaves (r.red.remove_all (r.inacc ++ r.acc)) gdt)
-        = gdt_eval gdt :=
-begin
-    induction gdt generalizing r ant,
-
-    case Gdt.branch {
-        ext env:1,
-        replace ha := congr_fun ha env,
-
-        -- branch to top
-        rw 𝒜' at ha,
-        rw ant_eval_all at ha,
-        rw ant_eval_all at ha,
-        rw map_ant at ha,
-        rw ←ant_eval_all at ha,
-        rw ←ant_eval_all at ha,
-        rw ←ant_eval_all at ha,
-
-        replace ha := inverse_map_ant_branch ha,
-        cases ha with ant1 ha,
-        cases ha with ant2 ha,
-        cases ha with ha1 ha,
-        cases ha with ha2 ha3,
-        rw ←ant_eval_all at ha2,
-        rw ←ant_eval_all at ha3,
-
-
-        rw ha1 at hr,
-        rw R at hr,
-        rw map_ant at hr,
-        rw R' at hr,
-        
-
-        set r1 := R' (map_ant is_empty.val ant1),
-        set r2 := R' (map_ant is_empty.val ant2),
-        replace hr : r = {acc := r1.acc ++ r2.acc, inacc := r1.inacc ++ r2.inacc, red := r1.red ++ r2.red} := hr,
-        
-        replace ha2: ant_eval_all ant1 = ant_eval_all (𝒜' gdt_tr1) := begin
-            ext env,
-            rw ha2,
-            --library_search,
-        end,
-        specialize gdt_ih_tr1 r1 ant1,
-        rw ← R at r1,
-        
+        rw gdt_build_branch_replace_right_env p,
+        simp [gdt_build_branch, gdt_eval_option],
     },
 end
-    
--/
-
 
 
 
